{
 "cells": [
  {
   "cell_type": "markdown",
   "id": "188d623d-79cb-4d7e-aaed-112bb84d8d33",
   "metadata": {},
   "source": [
    "$\\textbf{Assignment 1 Ian Dave Canlas - 23200047}$\n",
    "\n",
    "Instructions:\n",
    "- Use latex.\n",
    "- Write your latex in jupyter notebook.\n",
    "- Push your answer to your github account.\n",
    "- Deadline is 2 weeks before finals.\n",
    "- Fail to submit 2 weeks before finals is an automatic 5.0 for this assignment.\n",
    "- Each problem is 25 points.\n",
    "\n",
    "1. Recall the definition of a rational number, denoted as $\\mathbb{Q}$. Prove that the Euler's number $e = \\Sigma_{k=0}^\\infty \\frac{1}{k!} \\notin \\mathbb{Q}$. A factorial is defined as $k! = (k)(k-1)(k-2)(k-3)..., \\forall k \\in \\mathbb{Z}^+$, note that $0! = 1$. Furthermore, a sum notation $\\Sigma_{k=0}^\\infty k = 0+ 1 + 2 + 3 +....+...$\n",
    "\n",
    "Let's revisit the definition of rational numbers, represented as $\\mathbb{Q}$. We aim to demonstrate that Euler's number $e = \\sum_{k=0}^\\infty \\frac{1}{k!}$ does not belong to $\\mathbb{Q}$. In this context, a factorial is defined as $k! = k \\cdot (k-1) \\cdot (k-2) \\cdot (k-3) \\cdots$, for all positive integers $k$, noting that $0! = 1$. Additionally, the summation notation $\\sum_{k=0}^\\infty k = 0 + 1 + 2 + 3 + \\ldots$.\n",
    "Assuming $e = \\mathbb{Q}$, let $e = \\frac{a}{b}$ where $a,b \\in \\mathbb{Z}$ with no common factors (except 1) and $b \\neq 0$.\n",
    "\n",
    "\\begin{gather}\n",
    "e = \\sum_{k=0}^\\infty \\frac{1}{k} = 1 + \\frac{1}{1!} + \\frac{1}{2!} + \\frac{1}{3!} + \\frac{1}{4!} + \\ldots\n",
    "\\end{gather}\n",
    "\n",
    "We then multiply both sides by the factorial of $b$:\n",
    "\n",
    "\\begin{gather}\n",
    "b!e = b! \\left(1 + \\frac{1}{1!} + \\frac{1}{2!} + \\frac{1}{3!} + \\frac{1}{4!} + \\frac{1}{5!} + \\ldots\\right)\n",
    "\\end{gather}\n",
    "\n",
    "Since $k \\geq b$, every term in the series for $e$ has a factor of $b!$ in the denominator:\n",
    "\n",
    "\\begin{gather}\n",
    "\\frac{1}{k!} = \\frac{1}{k \\cdot (k-1) \\cdot (k-2) \\cdots (b+1)} \\cdot \\frac{1}{(b \\cdot (b-1) \\cdot (b-2) \\cdots 2 \\cdot 1)} = \\frac{1}{(b-1)(b-2) \\cdots k}\n",
    "\\end{gather}\n",
    "\n",
    "Substituting:\n",
    "\n",
    "\\begin{gather}\n",
    "b!e = b! \\left(1 + \\frac{1}{1!} + \\frac{1}{2!} + \\ldots + \\frac{1}{(b+1)!} + \\frac{1}{(b+2)!} + \\ldots\\right)\n",
    "\\end{gather}\n",
    "\n",
    "The terms $\\frac{1}{(b+1)!} + \\frac{1}{(b+2)!}$ are fractions with denominators greater than or equal to $b$. Therefore, all terms are integers since $b!e$ is the sum of an integer ($b!$) and a series of integers.\n",
    "\n",
    "However, $b!e$ is both the sum of an integer ($b!$) and a series of integers. The sum of integers remains an integer. This contradiction arises as $b!e$ is assumed to be a rational number, but it must be an integer.\n",
    "\n",
    "Hence, $e = \\sum_{k=0}^\\infty \\frac{1}{k!} \\notin \\mathbb{Q}$.\n",
    "\n",
    "\n",
    "2. Prove Minkowski's Inequality for sums, $\\forall \\ p>1, (a_k, b_k)>0$:\n",
    "\n",
    "\n",
    "\\begin{gather}\n",
    "\\begin{bmatrix}\n",
    "\\Sigma_{k=1}^n |a_k + b_k|^p\n",
    "\\end{bmatrix}^\\frac{1}{p}\n",
    "\\leq\n",
    "\\begin{bmatrix}\n",
    "\\Sigma_{k=1}^n |a_k|^p\n",
    "\\end{bmatrix}^\\frac{1}{p}\n",
    "+\n",
    "\\begin{bmatrix}\n",
    "\\Sigma_{k=1}^n |b_k|^p\n",
    "\\end{bmatrix}^\\frac{1}{p}\n",
    "\\end{gather}\n",
    "\n",
    "\\begin{gather}\n",
    "\\begin{aligned}\n",
    "\\left( \\sum_{k=1}^n |a_k + b_k|^p \\right)^{1/p} &\\leq \\left( \\sum_{k=1}^n |a_k|^p \\right)^{1/p} \\left( \\sum_{k=1}^n |b_k|^p \\right)^{1 - \\frac{1}{p}} \\\\\n",
    "&= \\left( \\sum_{k=1}^n |a_k|^p \\right)^{1/p} \\left( \\sum_{k=1}^n |b_k|^{\\frac{p}{p-1}} \\right)^{\\frac{1}{p-1}} \\\\\n",
    "&= \\left( \\sum_{k=1}^n |a_k|^p \\right)^{1/p} \\left( \\sum_{k=1}^n |b_k|^p \\right)^{\\frac{1}{p-1}}\n",
    "\\end{aligned} \\\\\n",
    "\\text{Now, let's apply Hölder's inequality:} \\\\\n",
    "\\sum_{k=1}^n |x_k y_k| \\leq \\left( \\sum_{k=1}^n |x_k|^p \\right)^{1/p} \\left( \\sum_{k=1}^n |y_k|^q \\right)^{1/q} \\\\\n",
    "\\text{where } q \\text{ is the conjugate exponent of } p, \\text{ given by } \\frac{1}{p} + \\frac{1}{q} = 1. \\\\\n",
    "\\text{Let } x_k = \\frac{|a_k|}{\\left(\\sum_{k=1}^n |a_k|^p \\right)^{1/p}} \\text{ and } y_k = \\frac{|b_k|}{\\left(\\sum_{k=1}^n |b_k|^p \\right)^{1/p}}. \\\\\n",
    "\\text{Then, we have } \\sum_{k=1}^n |x_k|^p = 1 \\text{ and } \\sum_{k=1}^n |y_k|^q = 1. \\\\\n",
    "\\text{Applying Hölder's inequality:} \\\\\n",
    "\\begin{aligned}\n",
    "\\sum_{k=1}^n \\left| \\frac{a_k}{\\left(\\sum_{k=1}^n |a_k|^p \\right)^{1/p}} + \\frac{b_k}{\\left(\\sum_{k=1}^n |b_k|^p \\right)^{1/p}} \\right|^p &\\leq \\left( \\sum_{k=1}^n |x_k|^p \\right)^{1/p} \\left( \\sum_{k=1}^n |y_k|^q \\right)^{1/q} \\\\\n",
    "\\left( \\sum_{k=1}^n |a_k + b_k|^p \\right)^{1/p} &\\leq \\left( \\sum_{k=1}^n |a_k|^p \\right)^{1/p} \\left( \\sum_{k=1}^n |b_k|^p \\right)^{1/q}\n",
    "\\end{aligned} \\\\\n",
    "\\text{Since } \\frac{1}{p} + \\frac{1}{q} = 1, \\text{ we have } q = \\frac{p}{p-1}. \\\\\n",
    "\\text{Hence,} \\\\\n",
    "\\begin{aligned}\n",
    "\\left( \\sum_{k=1}^n |a_k + b_k|^p \\right)^{1/p} &\\leq \\left( \\sum_{k=1}^n |a_k|^p \\right)^{1/p} \\left( \\sum_{k=1}^n |b_k|^p \\right)^{1 - \\frac{1}{p}} \\\\\n",
    "&= \\left( \\sum_{k=1}^n |a_k|^p \\right)^{1/p} \\left( \\sum_{k=1}^n |b_k|^{\\frac{p}{p-1}} \\right)^{\\frac{1}{p-1}} \\\\\n",
    "&= \\left( \\sum_{k=1}^n |a_k|^p \\right)^{1/p} \\left( \\sum_{k=1}^n |b_k|^p \\right)^{\\frac{1}{p-1}}\n",
    "\\end{aligned} \\\\\n",
    "\\text{Thus, we've shown Minkowski's Inequality for sums:} \\\\\n",
    "\\left( \\sum_{k=1}^n |a_k + b_k|^p \\right)^{1/p} \\leq \\left( \\sum_{k=1}^n |a_k|^p \\right)^{1/p} + \\left( \\sum_{k=1}^n |b_k|^p \\right)^{1/p}\n",
    "\\end{gather}\n",
    "\n",
    "\n",
    "\n",
    "3. Prove the triangle inequality $|x+y| \\leq |x| + |y|, \\forall (x,y) \\in \\mathbb{R}$\n",
    "\n",
    "Let's establish the validity of the triangle inequality $|x+y| \\leq |x| + |y|$, for all $(x,y) \\in \\mathbb{R}$.\n",
    "\\textbf{Case 1:} If $x \\geq 0$ and $y \\geq 0$, then we have:\n",
    "\n",
    "$|x+y| = x + y$, $|x| = x$, and $|y| = y$.\n",
    "\n",
    "Therefore, $x + y \\leq x + y$. The inequality holds for this case.\n",
    "\n",
    "\\textbf{Case 2:} For $x \\geq 0$ and $y < 0$:\n",
    "\n",
    "$x - y \\leq x + y$\n",
    "\n",
    "$-y \\leq x+y$\n",
    "\n",
    "Since $y \\geq 0$, the inequality holds for this case.\n",
    "\n",
    "\\textbf{Case 3:} For $x < 0$ and $y \\geq 0$:\n",
    "\n",
    "$y-x \\leq x + y$\n",
    "\n",
    "$-x \\leq x$\n",
    "\n",
    "Since $x \\geq 0$, the inequality holds for this case.\n",
    "\n",
    "\\textbf{Case 4:} For $x < 0$ and $y < 0$:\n",
    "\n",
    "$-(x+y) \\leq x+y$\n",
    "\n",
    "$x+y \\leq x+y$\n",
    "\n",
    "The inequality holds for this case as well.\n",
    "\n",
    "By examining all cases, it is evident that $|x+y| \\leq |x| + |y|$, for all $(x,y) \\in \\mathbb{R}$.\n",
    "\n",
    "\n",
    "\n",
    "4. Prove Sedrakayan's Lemma $\\forall u_i, v_i \\in \\mathbb{R}^+$:\n",
    "\\begin{gather}\n",
    "\\frac{(\\Sigma_{i=1}^n u_i)^2}{\\Sigma_{i=1}^n v_i}\n",
    "\\leq\n",
    "\\Sigma_{i=1}^n \\frac{(u_i)^2}{v_i}\n",
    "\\end{gather}\n",
    "\n",
    "\n",
    "Let's demonstrate Sedrakayan's Lemma for all positive real numbers $u_i$ and $v_i$:\n",
    "\n",
    "\\begin{gather}\n",
    "\\frac{(\\sum_{i=1}^n u_i)^2}{\\sum_{i=1}^n v_i}\n",
    "\\leq\n",
    "\\sum_{i=1}^n \\frac{(u_i)^2}{v_i}\n",
    "\\end{gather}\n",
    "\n",
    "Solution:\n",
    "\n",
    "To establish Sedrakayan's Lemma, we'll utilize the Cauchy-Schwarz Inequality, which states that for any sequences of real numbers $a_i$ and $b_i$, the following holds:\n",
    "\n",
    "\\begin{gather}\n",
    "(\\sum_{i=1}^n a_i b_i)^2 \\leq (\\sum_{i=1}^n a_i^2)(\\sum_{i=1}^n b_i^2)\n",
    "\\end{gather}\n",
    "\n",
    "We apply the Cauchy-Schwarz Inequality to $\\sqrt{v_i}$ and $\\frac{u_i}{\\sqrt{v_i}}$:\n",
    "\n",
    "\\begin{gather}\n",
    "(\\sum_{i=1}^n \\sqrt{v_i} \\cdot \\frac{u_i}{\\sqrt{v_i}})^2 \\leq (\\sum_{i=1}^n (\\sqrt{v_i})^2)(\\sum_{i=1}^n (\\frac{u_i}{\\sqrt{v_i}})^2)\n",
    "\\end{gather}\n",
    "\n",
    "Simplifying, we get:\n",
    "\n",
    "\\begin{gather}\n",
    "(\\sum_{i=1}^n u_i)^2 \\leq (\\sum_{i=1}^n v_i)(\\sum_{i=1}^n \\frac{u_i^2}{v_i})\n",
    "\\end{gather}\n",
    "\n",
    "Now, dividing both sides by $\\sum_{i=1}^n v_i$, we obtain:\n",
    "\n",
    "\\begin{gather}\n",
    "\\frac{(\\sum_{i=1}^n u_i)^2}{\\sum_{i=1}^n v_i} \\leq \\sum_{i=1}^n \\frac{u_i^2}{v_i}\n",
    "\\end{gather}\n",
    "\n",
    "Therefore, we have proven Sedrakayan's Lemma.\n",
    "\n"
   ]
  },
  {
   "cell_type": "markdown",
   "id": "1de33a92-7a6a-4624-a8c5-994644cffc20",
   "metadata": {},
   "source": [
    "1. Consider the functions $f(x) = 2x+1$, $g(x)=2y-1$, $j(x) = |f(x)+g(x)|$, and $h(x) = j(x)^2$, show for the following inequality that:\n",
    "\n",
    "\\begin{gather}\n",
    "\\sqrt{|f(x)|^2} \\geq \\sqrt{h(x)} - \\sqrt{|g(x)|^2}, \\forall (x,y) \\in \\mathbb{Z}^+\n",
    "\\end{gather}\n",
    "\n",
    "\n",
    "\n",
    "Solution:\n",
    "\n",
    "Given that $h(x) = j(x)^2$ and $j(x) = |f(x) + g(x)| = |2x + 1 + 2y - 1| = |2x + 2y| = 2|x + y|$, we can express $h(x)$ as:\n",
    "\n",
    "\\begin{gather}\n",
    "h(x) = (2|x + y|)^2 = 4(x + y)^2\n",
    "\\end{gather}\n",
    "\n",
    "Our task is to demonstrate that $2y \\geq 2|x + y|$ holds for all $(x, y) \\in \\mathbb{Z}^+$.\n",
    "\n",
    "This inequality holds because the absolute value function ensures that $|x + y|$ is non-negative, and doubling it maintains its equality or decreases it to $2y$."
   ]
  },
  {
   "cell_type": "markdown",
   "id": "997eb723-4112-443b-92d6-4f6734ea8e3b",
   "metadata": {},
   "source": [
    "2. Prove Sedrakayan's Lemma if $u_i, v_i$ are square roots of an even integers:\n",
    "\\begin{gather}\n",
    "\\frac{(\\Sigma_{i=1}^n u_i)^2}{\\Sigma_{i=1}^n v_i}\n",
    "\\leq\n",
    "\\Sigma_{i=1}^n \\frac{(u_i)^2}{v_i}\n",
    "\\end{gather}\n",
    "\n",
    "Solution:\n",
    "\n",
    "Given Sedrakayan's Lemma for square roots of even integers, we can use the fact that if $u_i, v_i$ are square roots of even integers, then $u_i^2, v_i$ are integers.\n",
    "\n",
    "Since $u_i^2, v_i$ are integers, we can directly apply Sedrakayan's Lemma:\n",
    "\n",
    "\\begin{gather}\n",
    "\\frac{(\\sum_{i=1}^n u_i^2)}{(\\sum_{i=1}^n v_i)} \\leq \\sum_{i=1}^n \\frac{u_i^2}{v_i}\n",
    "\\end{gather}\n",
    "\n",
    "This validates Sedrakayan's Lemma for square roots of even integers."
   ]
  }
 ],
 "metadata": {
  "kernelspec": {
   "display_name": "Python 3 (ipykernel)",
   "language": "python",
   "name": "python3"
  },
  "language_info": {
   "codemirror_mode": {
    "name": "ipython",
    "version": 3
   },
   "file_extension": ".py",
   "mimetype": "text/x-python",
   "name": "python",
   "nbconvert_exporter": "python",
   "pygments_lexer": "ipython3",
   "version": "3.8.16"
  }
 },
 "nbformat": 4,
 "nbformat_minor": 5
}
